toString and join added for arrays

interp/src/prheap.ml
@@ -58,6 +58,7 @@ let prprealloc = function
   | Coq_prealloc_array -> "Coq_prealloc_array"
   | Coq_prealloc_array_is_array -> "Coq_prealloc_array_is_array"
   | Coq_prealloc_array_proto -> "Coq_prealloc_array_proto"
+  | Coq_prealloc_array_proto_join -> "Coq_prealloc_array_proto_join"
   | Coq_prealloc_array_proto_pop -> "Coq_prealloc_array_proto_pop"
   | Coq_prealloc_array_proto_push -> "Coq_prealloc_array_proto_push"
   | Coq_prealloc_array_proto_to_string -> "Coq_prealloc_array_proto_to_string"
