coq/JsSyntax.v
@@ -278,7 +278,8 @@ Inductive prealloc :=
   | prealloc_array
   | prealloc_array_is_array
   | prealloc_array_proto
-  | prealloc_array_proto_to_string (* LATER: support *)
+  | prealloc_array_proto_to_string 
+  | prealloc_array_proto_join
   | prealloc_array_proto_pop
   | prealloc_array_proto_push
   | prealloc_string
